elo-coq/ProgressPreservation.v
@@ -6,7 +6,7 @@ From Elo Require Export Core.
 
 Definition well_typed_memory D (mt : list typ) (m : mem) :=
   length mt = length m /\
-  (forall i, D / mt / (empty, empty) |- (get_tm m i) is (get_typ mt i)).
+  (forall i, D / mt / empty |-- (get_tm m i) is (get_typ mt i)).
 
 Inductive extends' : list typ -> list typ -> Prop :=
   | extends_nil : forall mt,
@@ -59,136 +59,98 @@ Proof.
   induction mt; auto using extends'.
 Qed.
 
+Lemma memory_weakening : forall D mt mt' Gamma t T, 
+  mt extends mt' ->
+  D / mt' / Gamma |-- t is T ->  
+  D / mt  / Gamma |-- t is T.
+Proof.
+  intros * Hext Htype.
+  induction Htype; eauto using @typeof.
+  assert (i < length mt). { eauto using extends_length. }
+  erewrite extends_lookup; auto using T_Loc.
+Qed.
+
+Lemma context_weakening : forall D mt Gamma Gamma' t T,
+  Gamma includes Gamma' ->
+  D / mt / Gamma' |-- t is T ->
+  D / mt / Gamma  |-- t is T.
+Proof.
+  intros * Hinc Htype.
+  generalize dependent Gamma.
+  induction Htype; intros * Hinc;
+  eauto using @typeof, update_preserves_inclusion.
+Qed.
+
+Lemma context_weakening_empty : forall D mt Gamma t T,
+  D / mt / empty |-- t is T ->
+  D / mt / Gamma |-- t is T.
+Proof.
+  intros * Htype.
+  eapply (context_weakening _ _ _ empty); auto.
+  discriminate.
+Qed.
+
 Lemma assignment_preserves_memory_typing : forall D m mt t i,
-  i < length mt ->
+  i < length m ->
   well_typed_memory D mt m ->
-  D / mt / (empty, empty) |- t is (get_typ mt i) ->
+  D / mt / empty |-- t is (get_typ mt i) ->
   well_typed_memory D mt (set m i t).
 Proof.
   intros * Hi [Hlen Htype1] Htype2. split.
   - rewrite Hlen. apply set_preserves_length.
   - intros j. destruct (PeanoNat.Nat.eqb i j) eqn:E.
     + apply PeanoNat.Nat.eqb_eq in E. subst.
-      rewrite Hlen in *.
       erewrite (get_set_involutive TM_Nil); auto.
     + apply PeanoNat.Nat.eqb_neq in E. subst.
       erewrite (get_set_i_neq_j TM_Nil); auto.
 Qed.
 
-Lemma aux : forall id id' T T' D mt Delta Gamma,
-  id <> id' ->
-  (D / mt / (Delta, Gamma) |- TM_Id id is T <->
-  D / mt / (Delta, update Gamma id' T') |- TM_Id id is T).
-Proof.
-  intros *.
-Admitted.
-
-Lemma aux2 : forall id U V D mt Delta Gamma t T,
-  D / mt / (Delta, update (update Gamma id U) id V) |- t is T ->
-  D / mt / (Delta, update Gamma id V) |- t is T.
-Proof.
-Admitted.
-
-Lemma gamma_weakening : forall D mt Gamma Gamma' t T,
-  Gamma includes Gamma' ->
-  D / mt / (empty, Gamma') |- t is T ->
-  D / mt / (empty, Gamma)  |- t is T.
-Proof.
-  intros * Hinc Htype.
-  remember (empty, Gamma)  as Context.  
-  remember (empty, Gamma') as Context'.
-  generalize dependent Gamma.
-  induction Htype; intros * Hinc Hc; subst;
-  inversion HeqContext'; subst;
-  eauto using @typeof.
-  - inversion HeqContext'. subst.
-    unfold lookup, empty, Map.empty' in H.
-    discriminate H.
-  - eapply T_Call.
-    + apply H.
-    + apply (IHHtype1 eq_refl Gamma0 Hinc eq_refl).
-    + apply (IHHtype2 eq_refl Gamma0 Hinc eq_refl).
-  (* TODO : remover par do contexto *)
-Qed.
-
-(*
-Lemma weakening : ∀ Gamma Gamma' ST t T,
-     inclusion Gamma Gamma' →
-     Gamma ; ST ⊢ t \in T →
-     Gamma' ; ST ⊢ t \in T.
-Proof.
-  intros Gamma Gamma' ST t T H Ht.
-  generalize dependent Gamma'.
-  induction Ht; eauto using inclusion_update.
-Qed.
-Lemma weakening_empty : ∀ Gamma ST t T,
-     empty ; ST ⊢ t \in T →
-     Gamma ; ST ⊢ t \in T.
-Proof.
-  intros Gamma ST t T.
-  eapply weakening.
-  discriminate.
-Qed.
-*)
-
-Lemma substitution_preserves_typing : forall D mt Delta Gamma id t u T U,
-  D / mt / (Delta, update Gamma id U) |- t is T ->
-  D / mt / (empty, empty) |- u is U ->
-  D / mt / (Delta, Gamma) |- [id := u] t is T.
+Lemma substitution_preserves_typing : forall D mt Gamma id t u T U,
+  D / mt / (update Gamma id U) |-- t is T ->
+  D / mt / empty |-- u is U ->
+  D / mt / Gamma |-- [id := u] t is T.
 Proof.
   intros * Ht Hu.
   generalize dependent T.
   generalize dependent Gamma.
-  induction t;
-  intros Gamma T Ht;
+  induction t; intros * Ht;
   inversion Ht; simpl; subst;
   eauto using @typeof.
   - destruct String.eqb eqn:E.
     + apply String.eqb_eq in E. subst.
-      rewrite lookup_update_involutive in H4.
-      discriminate H4.
-    + apply String.eqb_neq in E.
-      eapply (aux n id); eauto.
+      rewrite lookup_update_involutive in H1.
+      inversion H1. subst.
+      apply context_weakening_empty. assumption.
+    + apply T_Id_Val.
+      rewrite <- H1.
+      apply String.eqb_neq in E.
+      symmetry. apply lookup_update_idempotent. assumption.
   - destruct String.eqb eqn:E.
     + apply String.eqb_eq in E. subst.
-      rewrite lookup_update_involutive in H4.
-      inversion H4. subst. auto.
-      admit.
+      apply context_weakening_empty.
+      rewrite lookup_update_involutive in H1.
+      inversion H1. subst.
+      assumption.
     + apply String.eqb_neq in E.
-      eapply (aux n id); eauto.
-  - destruct String.eqb eqn:E.
-    + apply String.eqb_eq in E. subst.
-      rewrite lookup_update_involutive in H4.
-      admit.
-    + apply String.eqb_neq in E.
-      eapply (aux n id); eauto.
-  - admit.
+      apply T_Id_Var.
+      rewrite <- H1.
+      symmetry. apply lookup_update_idempotent.
+      assumption.
   - apply T_LetVal.
-    specialize (IHt1 _ _ H6).
-    apply IHt1.
-    destruct String.eqb eqn:E.
-    + apply String.eqb_eq in E. subst.
-      eauto using aux2.
-    + apply String.eqb_neq in E.
-  - admit.
-Admitted.
-
-Lemma memory_weakening : forall D mt mt' Delta Gamma t T, 
-  D / mt' / (Delta, Gamma) |- t is T ->
-  mt extends mt' ->
-  D / mt  / (Delta, Gamma) |- t is T.
-Proof.
-  intros * Htype Hext.
-  induction Htype; eauto using @typeof.
-  assert (i < length mt). { eauto using extends_length.  }
-  erewrite extends_lookup; auto using T_Loc.
+    + auto.
+    + destruct String.eqb eqn:E in *.
+      * apply String.eqb_eq in E. subst.
+        eauto using context_weakening, update_overwrite.
+      * apply String.eqb_neq in E.
+        eauto using context_weakening, update_permutation.
+  - apply T_LetVar.
+    + auto.
+    + destruct String.eqb eqn:E in *.
+      * apply String.eqb_eq in E. subst.
+        eauto using context_weakening, update_overwrite.
+      * apply String.eqb_neq in E.
+        eauto using context_weakening, update_permutation.
 Qed.
-
-(* Lemma well_typed_memory_app : forall D mt m t T,
-  well_typed_memory D mt m ->
-  D / mt / (nil, nil) |- t is T ->
-  well_typed_memory D (mt ++ T :: nil) (m ++ t :: nil).
-Admitted. *)
 
 Lemma length_add : forall {A B} (l1 : list A) (l2 : list B) a b,
   length l1 = length l2 ->
@@ -197,113 +159,83 @@ Proof.
 Admitted.
 
 Theorem preservation : forall D D' m m' mt t t' T,
-  D / mt / (nil, nil) |- t is T ->
+  D / mt / empty |-- t is T ->
   well_typed_memory D mt m ->
   D / m / t --> D' / m' / t' ->
   exists mt',
     mt' extends mt /\
-    D' / mt' / (nil, nil) |- t' is T /\
+    D' / mt' / empty |-- t' is T /\
     well_typed_memory D' mt' m'.
 Proof.
-  remember (nil, nil) as Context.
+  remember empty as Gamma.
   intros * Htype.
   generalize dependent t'.
-  induction Htype; intros ?t' Hmem Hstep.
-  - inversion Hstep. (* T_Nil *)
-  - inversion Hstep. (* T_Num *)
-  - inversion Hstep. (* T_IdSharedVal *)
-  - inversion Hstep. (* T_IdLocalVal *)
-  - inversion Hstep. (* T_IdVar *)
-  - (* T_Asg *)
-    inversion Hstep; inversion HeqContext; subst.
-    + specialize (IHHtype2 eq_refl e' Hmem H6).
-      destruct IHHtype2 as [mt' [Hextends [Htype' Hmem']]].
-      exists mt'. split. apply Hextends. split.
-      * eauto using memory_weakening, T_Asg.
-      * auto.
-    + specialize (IHHtype1 eq_refl t'0 Hmem H7).
-      destruct IHHtype1 as [mt' [Hextends [Htype' Hmem']]].
-      exists mt'. split. apply Hextends. split.
-      * eauto using memory_weakening, T_Asg.
-      * auto.
-    + inversion Htype1. subst. exists mt. split.
-      * apply extends_refl.
-      * split.
-        { apply T_Nil. }
-        { apply assignment_preserves_memory_typing; auto. }
-  - (* T_Call *)
-    inversion Hstep; inversion HeqContext; subst.
-    + specialize (IHHtype1 eq_refl e' Hmem H7).
-      destruct IHHtype1 as [mt' [Hextends [Htype' Hmem']]].
-      exists mt'. split.
-      * auto.
-      * split.
-        { eapply T_Call; eauto using memory_weakening. }
-        { auto. }
-    + exists mt. split.
-      * apply extends_refl.
-      * split.
-        { rewrite H in H8. injection H8 as ?; subst.
-          eapply substitution_preserves_typing; eauto. }
-        { auto. }
-  - (* T_Seq *)
-    inversion Hstep; inversion HeqContext; subst.
-    + specialize (IHHtype1 eq_refl t2 Hmem H6).
-      destruct IHHtype1 as [mt' [Hextends [Htype' Hmem']]].
-      exists mt'. split.
-      * auto.
-      * split; eauto using T_Seq, memory_weakening.
-    + exists mt. split.
-      * apply extends_refl.
-      * split; assumption.
-  - (* T_LetVal *)
-    inversion Hstep; inversion HeqContext; subst.
-    + specialize (IHHtype1 eq_refl e' Hmem H8).
-      destruct IHHtype1 as [mt' [Hextends [Htype' Hmem']]].
-      exists mt'. split.
-      * assumption.
-      * split; try assumption.
-        eauto using T_LetVal, memory_weakening.
-    + exists (add mt A). split.
-      * apply extends_add.
-      * split.
-        { eapply substitution_preserves_typing.
-          assert (add mt A extends mt). { apply extends_add. }
-          eapply (memory_weakening _ _ _ _ _ _ _ Htype2 H).
-          admit.
-        }
-        { destruct Hmem as [Hlen H]. split.
-          - unfold m'1. apply length_add. auto.
-          - intros j. specialize (H j).
-            admit.
-        }
-  - (* T_LetVar *)
-    inversion Hstep; inversion HeqContext; subst.
-    + specialize (IHHtype1 eq_refl e' Hmem H9).
-      destruct IHHtype1 as [mt' [Hextends [Htype' Hmem']]].
-      exists mt'. split.
-      * assumption.
-      * split; try assumption.
-        eauto using T_LetVar, memory_weakening.
-    + exists (add mt A). split.
-      * apply extends_add.
-      * split.
-        { eapply substitution_preserves_typing.
-          assert (add mt A extends mt). { apply extends_add. }
-          eapply (memory_weakening _ _ _ _ _ _ _ Htype2 H).
-          admit.
-        }
-        { destruct Hmem as [Hlen H]. split.
-          - apply length_add. auto.
-          - intros j. specialize (H j).
-            admit.
-        }
-  - admit.
+  induction Htype; intros ?t' Hmem Hstep;
+  inversion Hstep; subst.
+  (* T_Asg *)
+  * eapply IHHtype2 in H6; auto.
+    destruct H6 as [mt' [Hext [Htype' Hmem']]].
+    exists mt'. split; try split; eauto using memory_weakening, T_Asg.
+  * eapply IHHtype1 in H7; auto.
+    destruct H7 as [mt' [Hext [Htype' Hmem']]].
+    exists mt'. split; try split; eauto using memory_weakening, T_Asg.
+  * exists mt. split. apply extends_refl. split. apply T_Nil.
+    eapply assignment_preserves_memory_typing; auto.
+    inversion Htype1. subst. eauto.
+  (* T_Call *)
+  * eapply IHHtype in H7; trivial.
+    destruct H7 as [mt' [Hextends [Htype' Hmem']]].
+    exists mt'. split; trivial.
+    split; try eapply T_Call; eauto using memory_weakening.
+  * exists mt. split; only 1 : apply extends_refl.
+    split; trivial. rewrite H in H8. injection H8 as ?; subst.
+    eapply substitution_preserves_typing.
+    ** admit.
+    ** apply Htype.
+  (* T_Seq *)
+  * specialize (IHHtype1 eq_refl t2 Hmem H6).
+    destruct IHHtype1 as [mt' [? [? ?]]].
+    exists mt'. split. assumption.
+    split; eauto using T_Seq, memory_weakening.
+  * exists mt. split. apply extends_refl. split; assumption.
+  (* T_LetVal *)
+  * specialize (IHHtype1 eq_refl e' Hmem H8).
+    destruct IHHtype1 as [mt' [Hextends [Htype' Hmem']]].
+    exists mt'. split. assumption.
+    split; eauto using T_LetVal, memory_weakening.
+  * exists mt. split.
+    ** apply extends_refl.
+    ** split. eapply substitution_preserves_typing.
+       *** apply Htype2.
+       *** destruct Hmem as [Hlen Hmem2].
+           specialize (Hmem2 i).
+           admit.
+       *** destruct Hmem as [Hlen H]. split.
+           admit. admit.
+  (* T_LetVar *)
+  * specialize (IHHtype1 eq_refl e' Hmem H8).
+    destruct IHHtype1 as [mt' [Hextends [Htype' Hmem']]].
+    exists mt'. split. assumption.
+    split; eauto using T_LetVar, memory_weakening.
+  * exists (add mt A). split.
+    ** apply extends_add.
+    ** split.
+      *** eapply substitution_preserves_typing.
+         assert (add mt A extends mt). { apply extends_add. }
+         eapply (memory_weakening _ _ _ _ _ _ H Htype2).
+         admit.
+      *** destruct Hmem as [Hlen H]. split.
+         **** apply length_add. auto.
+         **** intros j. specialize (H j).
+             admit.
+  * admit.
+  * admit.
+  * admit.
+  * admit.
 Admitted.
-(* Qed *)
 
 Theorem progress : forall D m mt t T,
-  D / mt / (nil, nil) |- t is T ->
+  D / mt / empty |-- t is T ->
   well_typed_memory D mt m ->
   (value t \/ exists D' m' t', D / m / t --> D' / m' / t').
 Admitted.
